Adjust to new way of handling uninterpreted function

books/projects/smtlink/verified/uninterpreted-fn-cp.lisp
@@ -22,251 +22,455 @@
 (include-book "ordinals/lexicographic-ordering" :dir :system)
 (set-state-ok t)
 
-(acl2::defevaluator-fast unev unev-lst
-                         ((if a b c) (equal a b) (not a)
-                          (cons a b) (binary-+ a b)
-                          (typespec-check ts x)
-                          (iff a b)
-                          (implies a b)
-                          (hint-please hint)
-                          (return-last x y z))
-                         :namedp t)
+(defsection uninterpreted-fn-cp
+  :parents (verified)
+  :short "Verified clause-processor for proving return types of uninterpreted
+  functions."
 
-(acl2::def-ev-theoremp unev)
-(acl2::def-meta-extract unev unev-lst)
-(acl2::def-unify unev unev-alist)
+  (acl2::defevaluator-fast unev unev-lst
+                           ((if a b c) (equal a b) (not a)
+                            (cons a b) (binary-+ a b)
+                            (typespec-check ts x)
+                            (iff a b)
+                            (implies a b)
+                            (hint-please hint)
+                            (return-last x y z)
+                            (binary-+ x y))
+                           :namedp t)
 
-(local
- (defthm unev-of-disjoin
-   (iff (unev (disjoin clause) a)
-        (acl2::or-list (unev-lst clause a)))
-   :hints(("Goal" :in-theory (enable acl2::or-list len)
-           :induct (len clause)))))
+  (acl2::def-ev-theoremp unev)
+  (acl2::def-meta-extract unev unev-lst)
+  (acl2::def-unify unev unev-alist)
 
-(define find-fixer ((term pseudo-termp)
-                    (func func-p)
-                    state)
-  :returns (the-fixer symbolp)
-  :guard (and (consp term)
-              (symbolp (car term)))
-  :guard-debug t
-  (b* ((term (pseudo-term-fix term))
-       (func (func-fix func))
-       (thms (func->meta-extract-thms func))
-       ((unless (and (consp thms)
-                     (car thms)
-                     (consp (cdr thms))
-                     (cadr thms)
-                     (null (cddr thms))))
-        (er hard? 'uninterpreted-fn-cp=>find-fixer "Smtlink need two theorems
+  (local
+   (defthm unev-of-disjoin
+     (iff (unev (disjoin clause) a)
+          (acl2::or-list (unev-lst clause a)))
+     :hints(("Goal" :in-theory (enable acl2::or-list len)
+             :induct (len clause)))))
+
+  (define type-thm-remove-lambda ((func func-p)
+                                  state)
+    :returns (type-thm pseudo-termp) ;; type-fix
+    (b* ((func (func-fix func))
+         (thms (func->meta-extract-thms func))
+         ((mv ok type-of-f)
+          (case-match thms
+            ((type-of-f &)
+             (mv t type-of-f))
+            (& (mv nil nil))))
+         ((unless ok)
+          (er hard? 'uninterpreted-fn-cp=>type-thm-remove-lambda "Smtlink need two theorems
  to justify the proof of return types of uninterpreted functions. Expected
  [type-of-f] and [type-fix-when-type], but got: ~q0" thms))
-       ((list type-of-f type-fix-when-type) thms)
-       (type-thm (acl2::meta-extract-formula-w type-of-f (w state)))
-       ((unless (and (consp type-thm)
-                     (pseudo-lambdap (car type-thm))
-                     (pseudo-term-listp (cdr type-thm))))
-        (er hard? 'uninterpreted-fn-cp=>find-fixer "Type theorem type-of-f is
+         (type-thm (acl2::meta-extract-formula-w type-of-f (w state)))
+         ((unless (and (pseudo-termp type-thm)
+                       (consp type-thm)
+                       (pseudo-lambdap (car type-thm))
+                       (pseudo-term-listp (cdr type-thm))))
+          (er hard? 'uninterpreted-fn-cp=>type-thm-remove-lambda "Type theorem type-of-f is
  not of the expected shape: ~q0" type-thm))
-       ((cons fn fn-actuals) type-thm)
-       (type-thm-w/o-lambda (lambda-substitution fn fn-actuals))
-       ((mv ok typep fn-call)
-        (case-match type-thm-w/o-lambda
-          ((typep fn-call)
-           (mv t typep fn-call))
-          (& (mv nil nil nil))))
-       ((unless (and ok (pseudo-termp fn-call) (symbolp typep)))
-        (er hard? 'uninterpreted-fn-cp=>find-fixer "Type theorem after
- substitution does not match expectation: ~q0" type-thm-w/o-lambda))
-       ((mv match-ok &)
-        (acl2::simple-one-way-unify fn-call term nil))
-       ((unless match-ok)
-        (er hard? 'uninterpreted-fn-cp=>find-fixer "Simple-one-way-unify
- failed: ~p0 and p1~%" fn-call term))
-       (fix-thm (acl2::meta-extract-formula-w type-fix-when-type (w state)))
-       ((unless (pseudo-termp fix-thm))
-        (er hard? 'uninterpreted-fn-cp=>find-fixer "Fix theorem is not a pseudo-termp: ~q0" fix-thm))
-       (formals (all-vars fix-thm))
-       ((unless (and (consp formals) (symbolp (car formals))
-                     (null (cdr formals))))
-        (er hard? 'uninterpreted-fn-cp=>find-fixer "Free vars from the fix
-                    theorem do ~p0 not match expectation: ~p1~%" fix-thm
-                    formals))
-       (fix-thm-substituted
-        (acl2::substitute-into-term fix-thm
-                                    (pairlis$ formals (list term))))
-       ((mv ok the-fixer)
-        (case-match fix-thm-substituted
-          (('implies (!typep !fn-call)
-                     ('equal (the-fixer !fn-call) !fn-call))
-           (mv t the-fixer))
-          (& (mv nil nil))))
-       ((unless (and ok (symbolp the-fixer)))
-        (er hard? 'uninterpreted-fn-cp=>find-fixer "Fixer theorem doesn't match expectation" fix-thm)))
-    the-fixer))
+         ((cons fn fn-actuals) type-thm)
+         (type-thm-w/o-lambda (lambda-substitution fn fn-actuals))
+         (- (cw "type-thm-w/o-lambda: ~q0" type-thm-w/o-lambda)))
+      type-thm-w/o-lambda))
 
-(skip-proofs
-(defthm find-fixer-correct
-  (implies (and (unev-meta-extract-global-facts)
-                (alistp a)
-                (pseudo-termp term)
-                (consp term)
-                (symbolp (car term)))
-           (or (null (find-fixer term func state))
-               (equal (unev (cons (find-fixer term func state)
-                                  (cons term nil))
-                            a)
-                      (unev term a))))
-  :hints (("Goal"
-           :do-not-induct t
-           :in-theory (e/d (find-fixer
-                            unev-of-fncall-args)
-                           (pseudo-term-listp
-                            pseudo-termp
-                            car-cdr-elim))
-           ))))
 
-(defines uninterpreted
-  :well-founded-relation l<
-  :flag-local nil
-  :flag-defthm-macro defthm-uninterpreted
-  :verify-guards nil
+    ;; BOZO: Should be able to do functional-instantiation of
+    ;; lambda-substitution-correct, but I got lost at the symbols from package acl2
+    ;; and current package
+    (local (defthm unev-alist-of-pairlis$
+             (equal (unev-alist (pairlis$ x y) a)
+                    (pairlis$ x (unev-lst y a)))))
 
-  (define uninterpreted-list ((term-lst pseudo-term-listp)
-                              (fn-lst func-alistp)
-                              (fty-info fty-info-alist-p)
-                              state)
-    :returns (new-term-lst pseudo-term-listp)
-    :measure (acl2-count (pseudo-term-list-fix term-lst))
-    :hints (("Goal" :in-theory (enable pseudo-term-list-fix
-                                       pseudo-term-fix)))
-    (b* ((term-lst (pseudo-term-list-fix term-lst))
-         ((unless (consp term-lst)) term-lst)
-         ((cons first rest) term-lst)
-         (first-term (uninterpreted first fn-lst fty-info state)))
-      (cons first-term
-            (uninterpreted-list rest fn-lst fty-info state))))
+    (defthm lambda-substitution-correct-uninterpreted
+      (implies (and (unev-meta-extract-global-facts)
+                    (alistp a)
+                    (pseudo-lambdap fn-call)
+                    (pseudo-term-listp fn-actuals))
+               (equal
+                (unev (lambda-substitution fn-call fn-actuals) a)
+                (unev (cons fn-call fn-actuals) a)))
+      :hints (("Goal"
+               :in-theory (enable lambda-substitution))))
 
-  (define uninterpreted ((term pseudo-termp)
-                         (fn-lst func-alistp)
-                         (fty-info fty-info-alist-p)
-                         state)
-    :returns (new-term pseudo-termp)
-    :measure (acl2-count (pseudo-term-fix term))
-    (b* ((term (pseudo-term-fix term))
-         ;; (fn-lst (func-alist-fix fn-lst))
-         ;; If first term is a symbolp or is quoted, return the current facts
-         ((if (or (acl2::variablep term) (acl2::fquotep term))) term)
-         ;; The first term is now a function call:
-         ;; Cons the function call and function actuals out of term
-         ((cons fn-call fn-actuals) term)
-         ;; If fn-call is a pseudo-lambdap, transform the body
-         ((if (pseudo-lambdap fn-call)) term)
-         ;; If fn-call is neither a lambda expression nor a function call
-         ((unless (mbt (symbolp fn-call))) nil)
+    (defthm type-thm-remove-lambda-correct
+      (implies (and (unev-meta-extract-global-facts)
+                    (alistp a))
+               (or (null (type-thm-remove-lambda func state))
+                   (unev (type-thm-remove-lambda func state) a)))
+      :hints (("Goal"
+               :do-not-induct t
+               :in-theory (e/d (type-thm-remove-lambda
+                                unev-of-fncall-args)
+                               (pseudo-term-listp
+                                pseudo-termp
+                                car-cdr-elim
+                                w
+                                lambda-substitution-correct-uninterpreted))
+               :use ((:instance
+                      lambda-substitution-correct-uninterpreted
+                      (a a)
+                      (fn-call
+                       (car (meta-extract-formula (car (func->meta-extract-thms func))
+                                                  state)))
+                      (fn-actuals
+                       (cdr (meta-extract-formula (car (func->meta-extract-thms func))
+                                                  state)))
+                      ))
+               )))
 
-         ;; -----------------------------------------------------------
-         ;; Now the term is a function call
-         (basic-function (member-equal fn-call *SMT-basics*))
-         (flex? (fncall-of-flextype fn-call fty-info))
-         ((if (or basic-function flex?)) term)
-         ;; fn-call is not a basic function nor a flex function
-         (user-defined (assoc-equal fn-call fn-lst))
-         ((unless user-defined) term)
-         (fixer (find-fixer term (cdr user-defined) state))
-         ((unless (and fixer (not (equal fixer 'quote)))) term))
-      (cons fixer (cons (cons fn-call (uninterpreted-list fn-actuals fn-lst
-                                                          fty-info state))
-                        nil))))
-  )
+    (define uninterpreted-substitution ((term pseudo-termp)
+                                        (type-thm pseudo-termp))
+      :returns (new-term pseudo-termp
+                         :hints (("Goal"
+                                  :in-theory (enable pseudo-termp
+                                                     pseudo-term-fix
+                                                     pairlis$))))
+      (b* ((term (pseudo-term-fix term))
+           (type-thm (pseudo-term-fix type-thm))
+           (vars (reverse (acl2::simple-term-vars type-thm)))
+           (- (cw "vars: ~q0" vars))
+           (- (cw "vars term: ~q0" term))
+           ((unless (and (consp term)
+                         (acl2::pseudo-term-substp (pairlis$ vars (cdr term)))))
+            (prog2$ (er hard? 'uninterpreted-fn-cp=>uninterpreted-substitution
+                        "acl2::simple-term-vars failed with ~p0
+                                    and ~p1" type-thm term)
+                    nil)))
+        (acl2::substitute-into-term type-thm (pairlis$ vars (cdr term)))))
 
-(encapsulate ()
-  (local
-   (defthm symbolp-of-car-of-pseudo-termp
-     (implies (and (consp term)
-                   (not (pseudo-lambdap (car term)))
-                   (pseudo-termp term))
-              (symbolp (car term)))
-     :hints (("Goal" :in-theory (enable pseudo-lambdap pseudo-termp))))
-   )
+    (define type-thm-full ((term pseudo-termp)
+                           (func func-p)
+                           state)
+      :returns (new-term pseudo-termp)
+      (b* ((term (pseudo-term-fix term))
+           (type-thm-w/o-lambda (type-thm-remove-lambda func state))
+           ((unless type-thm-w/o-lambda)
+            (prog2$ (er hard? 'uninterpreted-fn-cp=>type-thm-full
+                        "Something is wrong with type-thm-remove-lambda.")
+                    nil))
+           (type-thm (uninterpreted-substitution term type-thm-w/o-lambda))
+           ((unless type-thm)
+            (prog2$ (er hard? 'uninterpreted-fn-cp=>type-thm-full
+                        "Something is wrong with uninterpreted-substitution.")
+                    nil)))
+        type-thm))
 
-  (local
-   (defthm func-p-of-cdr-of-assoc-equal-of-func-alistp
-     (implies (and (func-alistp fn-lst)
-                   (assoc-equal (car term) fn-lst))
-              (and (consp (assoc-equal (car term) fn-lst))
-                   (func-p (cdr (assoc-equal (car term) fn-lst)))))))
+    (local (defthm alistp-of-unev-alist (alistp (unev-alist x a))))
 
-  (verify-guards uninterpreted)
-
-  (defthm-uninterpreted
-    (defthm uninterpreted-term
+    (defthm type-thm-full-correct
       (implies (and (unev-meta-extract-global-facts)
                     (alistp a)
                     (pseudo-termp term))
-               (equal (unev
-                       (uninterpreted term fn-lst fty-info state) a)
-                      (unev term a)))
-      :hints ('(:expand ((uninterpreted term fn-lst fty-info state))
-                        :in-theory (e/d (unev-of-fncall-args)
-                                        (find-fixer-correct))
-                        :use ((:instance find-fixer-correct
-                                         (term term)
-                                         (a a)
-                                         (func (cdr (assoc-equal (car term) fn-lst)))))))
-      :flag uninterpreted)
-    (defthm uninterpreted-term-lst
+               (or (null (type-thm-full term func state))
+                   (unev (type-thm-full term func state) a)))
+      :hints (("Goal"
+               :do-not-induct t
+               :in-theory (e/d (type-thm-full
+                                uninterpreted-substitution)
+                               (type-thm-remove-lambda-correct))
+               :use ((:instance type-thm-remove-lambda-correct
+                                (func func)
+                                (a (pairlis$
+                                    (reverse (acl2::simple-term-vars
+                                              (type-thm-remove-lambda func state)))
+                                    (unev-lst (cdr term) a)))))
+               )))
+
+
+    (define fix-thm-meta-extract ((func func-p)
+                                  state)
+      :returns (new-term pseudo-termp)
+      (b* ((func (func-fix func))
+           (thms (func->meta-extract-thms func))
+           ((mv ok type-fix-when-type)
+            (case-match thms
+              ((& type-fix-when-type)
+               (mv t type-fix-when-type))
+              (& (mv nil nil))))
+           ((unless ok)
+            (er hard? 'uninterpreted-fn-cp=>fix-thm-meta-extract "Smtlink need two theorems
+ to justify the proof of return types of uninterpreted functions. Expected
+ [type-of-f] and [type-fix-when-type], but got: ~q0" thms))
+           (- (cw "type-fix-when-type: ~q0" type-fix-when-type))
+           (fix-thm (acl2::meta-extract-formula-w type-fix-when-type (w
+                                                                      state)))
+           (- (cw "fix-thm1: ~q0" fix-thm))
+           ((unless (and (pseudo-termp fix-thm) (not (equal fix-thm ''t))))
+            (er hard? 'uninterpreted-fn-cp=>fix-thm-meta-extract "Type theorem
+                              type-of-f is not of the expected shape: ~q0"
+                fix-thm)))
+        fix-thm))
+
+    (defthm fix-thm-meta-extract-correct
+      (implies (and (unev-meta-extract-global-facts)
+                    (alistp a))
+               (or (null (fix-thm-meta-extract func state))
+                   (unev (fix-thm-meta-extract func state) a)))
+      :hints (("Goal"
+               :do-not-induct t
+               :in-theory (e/d (fix-thm-meta-extract
+                                unev-of-fncall-args)
+                               (pseudo-term-listp
+                                pseudo-termp
+                                car-cdr-elim
+                                w))
+               )))
+
+    (define fix-thm-full ((term pseudo-termp)
+                          (func func-p)
+                          state)
+      :returns (new-term pseudo-termp)
+      :guard-debug t
+      (b* ((term (pseudo-term-fix term))
+           (fix-thm (fix-thm-meta-extract func state))
+           ((unless fix-thm)
+            (er hard? 'uninterpreted-fn-cp=>fix-thm-full
+                "Something is wrong with fix-thm-meta-extract."))
+           (vars (reverse (acl2::simple-term-vars fix-thm)))
+           (- (cw "fix-thm: ~q0" fix-thm))
+           ((unless (and (consp vars) (null (cdr vars))))
+            (er hard? 'uninterpreted-fn-cp=>fix-thm-full
+                "Free vars from fix-thm: ~q0" vars)))
+        (acl2::substitute-into-term fix-thm (pairlis$ vars (list term)))))
+
+    (defthm fix-thm-full-correct
       (implies (and (unev-meta-extract-global-facts)
                     (alistp a)
-                    (pseudo-term-listp term-lst))
-               (equal (unev-lst
-                       (uninterpreted-list term-lst fn-lst fty-info state)
-                       a)
-                      (unev-lst term-lst a)))
-      :hints ('(:expand ((uninterpreted-list term-lst fn-lst fty-info state)
-                         (uninterpreted-list nil fn-lst fty-info state))))
-      :flag uninterpreted-list))
-  )
+                    (pseudo-termp term))
+               (or (null (fix-thm-full term func state))
+                   (unev (fix-thm-full term func state) a)))
+      :hints (("Goal"
+               :do-not-induct t
+               :in-theory (e/d (fix-thm-full)
+                               (fix-thm-meta-extract-correct))
+               :use ((:instance fix-thm-meta-extract-correct
+                                (func func)
+                                (a (list
+                                    (cons (car (reverse
+                                                (acl2::simple-term-vars
+                                                 (fix-thm-meta-extract func state))))
+                                          (unev term a))))))
+               )))
 
-(define uninterpreted-fn ((cl pseudo-term-listp)
-                          (smtlink-hint t)
-                          state)
-  :returns (new-term pseudo-term-list-listp)
-  (b* (((unless (pseudo-term-listp cl)) nil)
-       ((unless (smtlink-hint-p smtlink-hint)) (list cl))
-       ;; generate all fty related stuff
-       (flextypes-table (table-alist 'fty::flextypes-table (w state)))
-       ((unless (alistp flextypes-table)) (list cl))
-       (h1 (generate-fty-info-alist smtlink-hint flextypes-table))
-       (h2 (generate-fty-types-top h1 flextypes-table))
-       ((smtlink-hint h) h2)
-       (fn-lst (make-alist-fn-lst h.functions))
-       (new-term (uninterpreted (disjoin cl) fn-lst h.fty-info state))
-       (next-cp (if h.custom-p
-                    (cdr (assoc-equal 'uninterpreted-custom
-                                      *SMT-architecture*))
-                  (cdr (assoc-equal 'uninterpreted *SMT-architecture*))))
-       ((if (null next-cp)) (list cl))
-       (the-hint
-        `(:clause-processor (,next-cp clause ',h state)))
-       (hinted-goal `((hint-please ',the-hint) ,new-term)))
-    (list hinted-goal)))
+    (define find-fixer ((term pseudo-termp)
+                        (func func-p)
+                        state)
+      :returns (fixer pseudo-termp)
+      (b* ((type-thm (type-thm-full term func state))
+           ((unless type-thm)
+            (er hard? 'uninterpreted-fn-cp=>find-fixer
+                "Something is wrong with type-thm-full."))
+           (fix-thm (fix-thm-full term func state))
+           ((unless fix-thm)
+            (er hard? 'uninterpreted-fn-cp=>find-fixer
+                "Something is wrong with fix-thm-full."))
+           (- (cw "fix-thm: ~q0" fix-thm))
+           (- (cw "type-thm: ~q0" type-thm))
+           (- (cw "term: ~q0" term))
+           ((mv ok fixed type-thm term)
+            (case-match fix-thm
+              (('implies type-thm
+                         ('equal fixed term))
+               (mv t fixed type-thm term))
+              (& (mv nil nil nil nil))))
+           (- (cw "fixed: ~p0, type-thm: ~p1, term: ~p2~%" fixed type-thm term))
+           ((unless (and ok (pseudo-termp fixed)))
+            (er hard? 'uninterpreted-fn-cp=>find-fixer
+                "Fixer wrong: ~q0" fixed)))
+        fixed))
 
-(define uninterpreted-cp ((cl pseudo-term-listp)
-                          (hints t)
-                          state)
-  (b* ((fixed-clause (uninterpreted-fn cl hints state)))
-    (value fixed-clause)))
+    (defthm find-fixer-correct
+      (implies (and (unev-meta-extract-global-facts)
+                    (alistp a)
+                    (pseudo-termp term))
+               (or (null (find-fixer term func state))
+                   (equal (unev (find-fixer term func state) a)
+                          (unev term a))))
+      :hints (("Goal"
+               :in-theory (e/d (find-fixer
+                                unev-of-fncall-args)
+                               (pseudo-term-listp
+                                pseudo-termp
+                                car-cdr-elim
+                                w
+                                fix-thm-full-correct
+                                type-thm-full-correct))
+               :use ((:instance fix-thm-full-correct
+                                (a a)
+                                (term term)
+                                (func func))
+                     (:instance type-thm-full-correct
+                                (a a)
+                                (term term)
+                                (func func)))
+               )))
 
-(local (in-theory (enable uninterpreted-cp uninterpreted-fn)))
+    (defines uninterpreted
+      :well-founded-relation l<
+      :flag-local nil
+      :flag-defthm-macro defthm-uninterpreted
+      :verify-guards nil
 
-(defthm uninterpreted-fn-correct
-  (implies (and (unev-meta-extract-global-facts)
-                (pseudo-term-listp clause)
-                (alistp a)
-                (unev (conjoin-clauses
-                       (acl2::clauses-result
-                        (uninterpreted-cp clause hints state)))
-                      a))
-           (unev (disjoin clause) a))
-  :rule-classes :clause-processor)
+      (define uninterpreted-list ((term-lst pseudo-term-listp)
+                                  (fn-lst func-alistp)
+                                  (fty-info fty-info-alist-p)
+                                  state)
+        :returns (new-term-lst pseudo-term-listp)
+        :measure (acl2-count (pseudo-term-list-fix term-lst))
+        :hints (("Goal" :in-theory (enable pseudo-term-list-fix
+                                           pseudo-term-fix)))
+        (b* ((term-lst (pseudo-term-list-fix term-lst))
+             ((unless (consp term-lst)) term-lst)
+             ((cons first rest) term-lst)
+             (first-term (uninterpreted first fn-lst fty-info state)))
+          (cons first-term
+                (uninterpreted-list rest fn-lst fty-info state))))
+
+      (define uninterpreted ((term pseudo-termp)
+                             (fn-lst func-alistp)
+                             (fty-info fty-info-alist-p)
+                             state)
+        :returns (new-term pseudo-termp)
+        :measure (acl2-count (pseudo-term-fix term))
+        (b* ((term (pseudo-term-fix term))
+             ;; (fn-lst (func-alist-fix fn-lst))
+             ;; If first term is a symbolp or is quoted, return the current facts
+             ((if (or (acl2::variablep term) (acl2::fquotep term))) term)
+             ;; The first term is now a function call:
+             ;; Cons the function call and function actuals out of term
+             ((cons fn-call fn-actuals) term)
+             ;; If fn-call is a pseudo-lambdap, transform the body
+             ((if (pseudo-lambdap fn-call))
+              (prog2$ (er hard? 'uninterpreted-fn-cp=>uninterpreted "There still
+                           exists lambda in the term. Very strange.~%~q0~%" term)
+                      term))
+             ;; If fn-call is neither a lambda expression nor a function call
+             ((unless (mbt (symbolp fn-call))) nil)
+             ((if (equal fn-call 'type-hyp)) term)
+
+             ;; -----------------------------------------------------------
+             ;; Now the term is a function call
+             (basic-function (member-equal fn-call *SMT-basics*))
+             (flex? (fncall-of-flextype fn-call fty-info))
+             ((if (or basic-function flex?))
+              (cons fn-call
+                    (uninterpreted-list fn-actuals fn-lst fty-info state)))
+             ;; fn-call is not a basic function nor a flex function
+             (user-defined (assoc-equal fn-call fn-lst))
+             ((unless user-defined)
+              (prog2$ (er hard? 'uninterpreted-fn-cp=>uninterpreted "User hasn't
+defined the uninterpreted function: ~q0" fn-call)
+                      term))
+             (fixed (find-fixer term (cdr user-defined) state))
+             ((mv ok fixer)
+              (case-match fixed
+                ((fixer (!fn-call . !fn-actuals))
+                 (mv t fixer))
+                (& (mv nil nil))))
+             ((unless (and ok (symbolp fixer)
+                           (not (equal fixer 'quote))))
+              (prog2$ (er hard? 'uninterpreted-fn-cp=>uninterpreted "Fixer wrong: ~q0" fixer)
+                      term)))
+          (list fixer
+                (cons fn-call (uninterpreted-list fn-actuals fn-lst
+                                                  fty-info state)))))
+      )
+
+    (encapsulate ()
+      (local
+       (defthm symbolp-of-car-of-pseudo-termp
+         (implies (and (consp term)
+                       (not (pseudo-lambdap (car term)))
+                       (pseudo-termp term))
+                  (symbolp (car term)))
+         :hints (("Goal" :in-theory (enable pseudo-lambdap pseudo-termp))))
+       )
+
+      (local
+       (defthm func-p-of-cdr-of-assoc-equal-of-func-alistp
+         (implies (and (func-alistp fn-lst)
+                       (assoc-equal (car term) fn-lst))
+                  (and (consp (assoc-equal (car term) fn-lst))
+                       (func-p (cdr (assoc-equal (car term) fn-lst)))))))
+
+      (verify-guards uninterpreted)
+
+      (defthm-uninterpreted
+        (defthm uninterpreted-term
+          (implies (and (unev-meta-extract-global-facts)
+                        (alistp a)
+                        (pseudo-termp term))
+                   (equal (unev
+                           (uninterpreted term fn-lst fty-info state) a)
+                          (unev term a)))
+          :hints ('(:expand ((uninterpreted term fn-lst fty-info state))
+                            :in-theory (e/d (unev-of-fncall-args)
+                                            (find-fixer-correct
+                                             member-equal
+                                             pseudo-term-listp
+                                             pseudo-termp
+                                             acl2::member-of-cons))
+                            :use ((:instance find-fixer-correct
+                                             (term term)
+                                             (a a)
+                                             (func (cdr (assoc-equal (car term) fn-lst)))))))
+          :flag uninterpreted)
+        (defthm uninterpreted-term-lst
+          (implies (and (unev-meta-extract-global-facts)
+                        (alistp a)
+                        (pseudo-term-listp term-lst))
+                   (equal (unev-lst
+                           (uninterpreted-list term-lst fn-lst fty-info state)
+                           a)
+                          (unev-lst term-lst a)))
+          :hints ('(:expand ((uninterpreted-list term-lst fn-lst fty-info state)
+                             (uninterpreted-list nil fn-lst fty-info state))))
+          :flag uninterpreted-list))
+      )
+
+    (define uninterpreted-fn ((cl pseudo-term-listp)
+                              (smtlink-hint t)
+                              state)
+      :returns (new-term pseudo-term-list-listp)
+      (b* (((unless (pseudo-term-listp cl)) nil)
+           (- (cw "cl: ~q0" cl))
+           ((unless (smtlink-hint-p smtlink-hint)) (list cl))
+           ;; generate all fty related stuff
+           (flextypes-table (table-alist 'fty::flextypes-table (w state)))
+           ((unless (alistp flextypes-table)) (list cl))
+           (h1 (generate-fty-info-alist smtlink-hint flextypes-table))
+           (h2 (generate-fty-types-top h1 flextypes-table))
+           ((smtlink-hint h) h2)
+           (fn-lst (make-alist-fn-lst h.functions))
+           (new-term (uninterpreted (disjoin cl) fn-lst h.fty-info state))
+           (next-cp (if h.custom-p
+                        (cdr (assoc-equal 'uninterpreted-custom
+                                          *SMT-architecture*))
+                      (cdr (assoc-equal 'uninterpreted *SMT-architecture*))))
+           ((if (null next-cp)) (list cl))
+           (the-hint
+            `(:clause-processor (,next-cp clause ',h state)))
+           (hinted-goal `((hint-please ',the-hint) ,new-term)))
+        (list hinted-goal)))
+
+    (define uninterpreted-fn-cp ((cl pseudo-term-listp)
+                                 (hints t)
+                                 state)
+      (b* ((fixed-clause (uninterpreted-fn cl hints state)))
+        (value fixed-clause)))
+
+    (local (in-theory (enable uninterpreted-fn-cp uninterpreted-fn)))
+
+    (defthm uninterpreted-fn-correct
+      (implies (and (unev-meta-extract-global-facts)
+                    (pseudo-term-listp clause)
+                    (alistp a)
+                    (unev (conjoin-clauses
+                           (acl2::clauses-result
+                            (uninterpreted-fn-cp clause hints state)))
+                          a))
+               (unev (disjoin clause) a))
+      :rule-classes :clause-processor)
+    )
