books/projects/smtlink/package.lsp
@@ -61,6 +61,10 @@
       sublis-var
       sublis-var1
       sublis-var1-lst
+      bool-fix
+      realfix
+      rfix
+      ifix
 
       read-string
 
